state/experiments/shared_in_pulse/SharedInPulse.fst
@@ -1,0 +1,56 @@
+module SharedInPulse
+
+
+open Pulse.Lib.Pervasives
+
+module H = PulseCore.Heap
+module GR = Pulse.Lib.MonotonicGhostRef
+open FStar.Preorder
+open Pulse.Lib.Stick
+
+type addr = nat
+let addr_of = H.core_ref_as_addr
+
+type map_sharedT = 
+  GR.mref #(addr -> bool) (fun (m0 m1:addr -> bool) -> forall p. m0 p ==> m1 p)
+
+noeq
+type sigT = {
+  map_shared : map_sharedT;
+  is_shared : #a:Type0 -> ref a -> slprop; (** one should add back here monotonic references.  *)
+  // is_shared_stable : #a:Type0 -> r:ref a -> Lemma (stable (is_shared r) (fun _ _ -> True)) [SMTPat (is_shared r)];
+
+  share : #a:Type0 -> sr:(ref a) -> #v:erased a -> #ms:erased (addr -> bool) ->
+    stt_ghost unit 
+      (* invariants *)
+      FStar.GhostSet.empty 
+
+      (* requires *)
+      (
+        pts_to sr v **
+        GR.pts_to map_shared #1.0R ms ** (** no idea how this work **)
+        // *addr_of sr =!= addr_of map_shared) (** we should not need this anymore, since map_share is ghost **)
+
+        //(forall p. p >= next_addr h0 ==> ~(sel h0 map_shared p)))) (** necessary to prove that freshly allocated references are not shared **)       
+        (forall* r. (forall* v. not* (pts_to r v) @==> ~(is_shared r)))
+      ) 
+
+
+      
+      (* ensures *)
+      (fun _ -> emp)
+      //   h0 `contains` sr /\
+      //   h0 `contains` map_shared /\
+      //   (addr_of sr =!= addr_of map_shared) /\ (** prevent sharing the map *)
+      //   ~(is_shared (map_shared) h0) /\
+      //   (forall p. p >= next_addr h0 ==> ~(sel h0 map_shared p)))) (** necessary to prove that freshly allocated references are not shared **)
+      // (ensures (fun h0 _ h1 ->
+      //   modifies !{map_shared} h0 h1 /\
+      //   ~(is_shared (map_shared) h1) /\
+      //   (forall b (r:ref b). is_shared r h0 ==> is_shared r h1) /\
+      //   (forall b (r:ref b). ~(is_shared r h0) /\ addr_of r =!= addr_of sr ==> ~(is_shared r h1)) /\
+      //   (forall p. p >= next_addr h1 ==> ~(sel h1 map_shared p)) /\
+      //   is_shared sr h1))
+}
+
+let pulse_five_in_fstar = five ()
